feat(Logic): Semantics.Meaningful

Logic/Logic/Semantics.lean
@@ -25,7 +25,7 @@ infix:45 " ⊧ " => Realize
 
 section
 
-variable (M F)
+variable (M)
 
 protected class Top where
   realize_top (𝓜 : M) : 𝓜 ⊧ (⊤ : F)
@@ -33,7 +33,7 @@ protected class Top where
 protected class Bot where
   realize_bot (𝓜 : M) : ¬𝓜 ⊧ (⊥ : F)
 
-class Tarski extends Semantics.Top M F, Semantics.Bot M F where
+class Tarski extends Semantics.Top M, Semantics.Bot M where
   realize_not (𝓜 : M) (p : F) : 𝓜 ⊧ ~p ↔ ¬𝓜 ⊧ p
   realize_imp {𝓜 : M} {p q : F} : 𝓜 ⊧ p ⟶ q ↔ (𝓜 ⊧ p → 𝓜 ⊧ q)
   realize_and {𝓜 : M} {p q : F} : 𝓜 ⊧ p ⋏ q ↔ 𝓜 ⊧ p ∧ 𝓜 ⊧ q
@@ -47,9 +47,9 @@ attribute [simp]
   Tarski.realize_and
   Tarski.realize_or
 
-variable {M F}
+variable {M}
 
-variable [Tarski M F]
+variable [Tarski M]
 
 variable {𝓜 : M}
 
@@ -80,24 +80,34 @@ variable (M)
 
 def Valid (f : F) : Prop := ∀ 𝓜 : M, 𝓜 ⊧ f
 
-def VaridSet (T : Set F) : Prop := ∀ 𝓜 : M, 𝓜 ⊧* T
+def Satisfiable (T : Set F) : Prop := ∃ 𝓜 : M, 𝓜 ⊧* T
 
-def Satisfiable (f : F) : Prop := ∃ 𝓜 : M, 𝓜 ⊧ f
-
-def SatisfiableSet (T : Set F) : Prop := ∃ 𝓜 : M, 𝓜 ⊧* T
-
-def modelOf (T : Set F) : Set M := {𝓜 | 𝓜 ⊧* T}
+def models (T : Set F) : Set M := {𝓜 | 𝓜 ⊧* T}
 
 variable {M}
+
+def theory (𝓜 : M) : Set F := {f | 𝓜 ⊧ f}
+
+class Meaningful (𝓜 : M) : Prop where
+  exists_unrealize : ∃ f, ¬𝓜 ⊧ f
+
+instance [Semantics.Bot M] (𝓜 : M) : Meaningful 𝓜 := ⟨⟨⊥, by simp⟩⟩
+
+lemma meaningful_iff {𝓜 : M} : Meaningful 𝓜 ↔ ∃ f, ¬𝓜 ⊧ f :=
+  ⟨by rintro ⟨h⟩; exact h, fun h ↦ ⟨h⟩⟩
+
+lemma not_meaningful_iff (𝓜 : M) : ¬Meaningful 𝓜 ↔ ∀ f, 𝓜 ⊧ f := by simp [meaningful_iff]
 
 lemma realizeSet_iff {𝓜 : M} {T : Set F} : 𝓜 ⊧* T ↔ ∀ ⦃f⦄, f ∈ T → Realize 𝓜 f :=
   ⟨by rintro ⟨h⟩; exact h, by intro h; exact ⟨h⟩⟩
 
-lemma valid_neg_iff [Tarski M F] (f : F) : Valid M (~f) ↔ ¬Satisfiable M f := by simp [Valid, Satisfiable]
+lemma not_satisfiable_finset [Tarski M] [DecidableEq F] (t : Finset F) :
+    ¬Satisfiable M (t : Set F) ↔ Valid M (t.image (~·)).disj := by
+  simp [Satisfiable, realizeSet_iff, Valid, Finset.map_disj]
 
-lemma not_satisfiable_finset [Tarski M F] [DecidableEq F] (t : Finset F) :
-    ¬SatisfiableSet M (t : Set F) ↔ Valid M (t.image (~·)).disj := by
-  simp [SatisfiableSet, realizeSet_iff, Valid, Finset.map_disj]
+lemma satisfiableSet_iff_models_nonempty {T : Set F} :
+    Satisfiable M T ↔ (models M T).Nonempty :=
+  ⟨by rintro ⟨𝓜, h𝓜⟩; exact ⟨𝓜, h𝓜⟩, by rintro ⟨𝓜, h𝓜⟩; exact ⟨𝓜, h𝓜⟩⟩
 
 namespace RealizeSet
 
@@ -113,6 +123,9 @@ lemma of_subset' {T U : Set F} {𝓜 : M} [𝓜 ⊧* U] (ss : T ⊆ U) : 𝓜 �
 instance empty' (𝓜 : M) : 𝓜 ⊧* (∅ : Set F) := ⟨fun p => by simp⟩
 
 @[simp] lemma empty (𝓜 : M) : 𝓜 ⊧* (∅ : Set F) := ⟨fun p => by simp⟩
+
+@[simp] lemma singleton_iff {f : F} {𝓜 : M} :
+    𝓜 ⊧* {f} ↔ 𝓜 ⊧ f := by simp [realizeSet_iff]
 
 @[simp] lemma insert_iff {T : Set F} {f : F} {𝓜 : M} :
     𝓜 ⊧* insert f T ↔ 𝓜 ⊧ f ∧ 𝓜 ⊧* T := by
@@ -136,7 +149,9 @@ instance empty' (𝓜 : M) : 𝓜 ⊧* (∅ : Set F) := ⟨fun p => by simp⟩
 
 end RealizeSet
 
-lemma SatisfiableSet.of_subset {T U : Set F} (h : SatisfiableSet M U) (ss : T ⊆ U) : SatisfiableSet M T :=
+lemma valid_neg_iff [Tarski M] (f : F) : Valid M (~f) ↔ ¬Satisfiable M {f} := by simp [Valid, Satisfiable]
+
+lemma Satisfiable.of_subset {T U : Set F} (h : Satisfiable M U) (ss : T ⊆ U) : Satisfiable M T :=
   by rcases h with ⟨𝓜, h⟩; exact ⟨𝓜, RealizeSet.of_subset h ss⟩
 
 variable (M)
@@ -145,7 +160,7 @@ instance [Semantics M F] : Semantics (Set M) F := ⟨fun s f ↦ ∀ 𝓜 ∈ s,
 
 @[simp] lemma empty_models (f : F) : (∅ : Set M) ⊧ f := by rintro h; simp
 
-abbrev Consequence (T : Set F) (f : F) : Prop := modelOf M T ⊧ f
+abbrev Consequence (T : Set F) (f : F) : Prop := models M T ⊧ f
 
 -- note that ⊨ (\vDash) is *NOT* ⊧ (\models)
 notation T:45 " ⊨[" M "] " p:46 => Consequence M T p
@@ -154,16 +169,25 @@ variable {M}
 
 lemma set_models_iff {s : Set M} : s ⊧ f ↔ ∀ 𝓜 ∈ s, 𝓜 ⊧ f := iff_of_eq rfl
 
-instance [Semantics.Top M F] : Semantics.Top (Set M) F := ⟨fun s ↦ by simp [set_models_iff]⟩
+instance [Semantics.Top M] : Semantics.Top (Set M) := ⟨fun s ↦ by simp [set_models_iff]⟩
+
+lemma set_meaningful_iff_nonempty [∀ 𝓜 : M, Meaningful 𝓜] {s : Set M} : Meaningful s ↔ s.Nonempty :=
+  ⟨by rintro ⟨f, hf⟩; by_contra A; rcases Set.not_nonempty_iff_eq_empty.mp A; simp at hf,
+   by rintro ⟨𝓜, h𝓜⟩
+      rcases Meaningful.exists_unrealize (𝓜 := 𝓜) with ⟨f, hf⟩
+      exact ⟨f, by simp [set_models_iff]; exact ⟨𝓜, h𝓜, hf⟩⟩⟩
+
+lemma meaningful_iff_satisfiableSet [∀ 𝓜 : M, Meaningful 𝓜] : Satisfiable M T ↔ Meaningful (models M T) := by
+  simp [set_meaningful_iff_nonempty, satisfiableSet_iff_models_nonempty]
 
 lemma consequence_iff {T : Set F} {f} : T ⊨[M] f ↔ ∀ {𝓜 : M}, 𝓜 ⊧* T → 𝓜 ⊧ f := iff_of_eq rfl
 
 lemma consequence_iff' {T : Set F} {f : F} : T ⊨[M] f ↔ (∀ (𝓜 : M) [𝓜 ⊧* T], 𝓜 ⊧ f) :=
   ⟨fun h _ _ => consequence_iff.mp h inferInstance, fun H 𝓜 hs => @H 𝓜 hs⟩
 
-lemma consequence_iff_not_satisfiable [Tarski M F] {f : F} :
-    T ⊨[M] f ↔ ¬SatisfiableSet M (insert (~f) T) := by
-  simp [consequence_iff, SatisfiableSet]; constructor
+lemma consequence_iff_not_satisfiable [Tarski M] {f : F} :
+    T ⊨[M] f ↔ ¬Satisfiable M (insert (~f) T) := by
+  simp [consequence_iff, Satisfiable]; constructor
   · intro h 𝓜 hf hT; have : 𝓜 ⊧ f := h hT; contradiction
   · intro h 𝓜; contrapose; exact h 𝓜
 
@@ -171,8 +195,6 @@ lemma weakening {T U : Set F} {f} (h : T ⊨[M] f) (ss : T ⊆ U) : U ⊨[M] f :
   consequence_iff.mpr fun hs => consequence_iff.mp h (RealizeSet.of_subset hs ss)
 
 lemma of_mem {T : Set F} {f} (h : f ∈ T) : T ⊨[M] f := fun _ hs => hs.RealizeSet h
-
-def theory (𝓜 : M) : Set F := {p | 𝓜 ⊧ p}
 
 end Semantics
 
@@ -211,7 +233,7 @@ variable (M F)
 
 class Compact : Prop where
   compact {T : Set F} :
-    Semantics.SatisfiableSet M T ↔ (∀ u : Finset F, ↑u ⊆ T → Semantics.SatisfiableSet M (u : Set F))
+    Semantics.Satisfiable M T ↔ (∀ u : Finset F, ↑u ⊆ T → Semantics.Satisfiable M (u : Set F))
 
 variable {F}
 
@@ -221,19 +243,19 @@ variable [Compact M F]
 
 variable {𝓜 : M}
 
-lemma conseq_compact [Semantics.Tarski M F] [DecidableEq F] {f : F} :
+lemma conseq_compact [Semantics.Tarski M] [DecidableEq F] {f : F} :
     T ⊨[M] f ↔ ∃ u : Finset F, ↑u ⊆ T ∧ u ⊨[M] f := by
   simp [Semantics.consequence_iff_not_satisfiable, compact (T := insert (~f) T)]
   constructor
   · intro ⟨u, ss, hu⟩
     exact ⟨Finset.erase u (~f), by simp [ss],
-      by simp; intro h; exact hu (Semantics.SatisfiableSet.of_subset h (by simp))⟩
+      by simp; intro h; exact hu (Semantics.Satisfiable.of_subset h (by simp))⟩
   · intro ⟨u, ss, hu⟩
     exact ⟨insert (~f) u,
       by simpa using Set.insert_subset_insert ss, by simpa using hu⟩
 
 lemma compact_cumulative {T : ℕ → Set F} (hT : Cumulative T) :
-    Semantics.SatisfiableSet M (⋃ s, T s) ↔ ∀ s, Semantics.SatisfiableSet M (T s) :=
+    Semantics.Satisfiable M (⋃ s, T s) ↔ ∀ s, Semantics.Satisfiable M (T s) :=
   ⟨by intro H s
       exact H.of_subset (Set.subset_iUnion T s),
    by intro H
